pancake/semantics/timeSemScript.sml
@@ -322,7 +322,7 @@ Definition steps_def:
   (steps prog [] m n s [] ⇔
    n < m  ∧
    (case s.waitTime of
-    | SOME w => w ≠ n ∧ w < m
+    | SOME w => w ≠ 0 ∧ w < m
     | NONE => T)) ∧
   (steps prog (lbl::lbls) m n s (st::sts) ⇔
      step prog lbl m n s st ∧
